matching-logic/src/Evaluation/Demo.v
@@ -1,0 +1,238 @@
+From Coq Require Import String.
+
+From MatchingLogic Require Import
+    Logic
+    ProofMode.MLPM
+    FreshnessManager
+    Theories.Definedness_Syntax
+    Theories.Definedness_ProofSystem.
+
+Import
+  MatchingLogic.Logic.Notations
+  MatchingLogic.DerivedOperators_Syntax.Notations
+  MatchingLogic.Theories.Definedness_Syntax.Notations.
+
+Open Scope string_scope.
+Open Scope list_scope.
+Open Scope ml_scope.
+
+Section running.
+  Notation definedness_theory := Theories.Definedness_Syntax.theory.
+  Notation definedness_syntax := Theories.Definedness_Syntax.Syntax.
+  Context
+    {Σ         : Signature}
+    {defsyntax : definedness_syntax}
+    (Γ         : Theory)
+    (HΓ        : definedness_theory ⊆ Γ).
+
+  Context
+    (f g P : Pattern)
+    (wff   : well_formed (ex, f))
+    (wfg   : well_formed (ex, g))
+    (wfP   : well_formed P)
+    (mfP   : mu_free P)
+    (x     : evar).
+
+  (*
+     Γ ⊢ (∀z.g z = f z) ∧ P (f x) → ∃y. P (g y)
+  *)
+  Lemma running_low :
+    Γ ⊢ (all, (g =ml f)) and P $ f^{evar:0 ↦ x} ---> 
+        ex, (P $ g).
+  Proof.
+    eapply prf_weaken_conclusion_meta_meta. 1-3: shelve.
+    * gapply (Ex_quan _ _ x). 1-2: shelve.
+    * cbn. rewrite bevar_subst_not_occur; [shelve|].
+      apply lhs_from_and. 1-3: shelve.
+      eapply prf_strenghten_premise_meta_meta.
+      4: gapply (forall_variable_substitution _ _ x). 1-5: shelve.
+      remember (fresh_evar P) as y.
+      remember ({| pcEvar := y; pcPattern := P $ patt_free_evar y |}) as C.
+      epose proof (equality_elimination_basic Γ (g^{evar:0 ↦ x}) (f^{evar:0 ↦ x})
+                                              C _ _ _ _ _).
+      subst C. cbn in H.
+      destruct decide in H. 2: congruence.
+      repeat rewrite free_evar_subst_no_occurrence in H. 1-2: shelve.
+      eapply prf_weaken_conclusion_meta_meta in H. 2-4: shelve.
+      - exact H.
+      - eapply prf_strenghten_premise_meta_meta. 1-3: shelve.
+        + gapply pf_conj_elim_r. 1-3: shelve.
+        + gapply A_impl_A. 1-2: shelve.
+
+  Unshelve.
+    (* 32 subgoals *)
+    (* 4 proof info goals *)
+    4,13,28,31: try_solve_pile.
+    (* 1 mu_free goal: *)
+    17: subst C; cbn; rewrite mfP; auto.
+    (* 2 free variable inclusion goal *)
+    17-18: subst y; solve_fresh.
+    (* 25 well_formed goals *)
+    1-25: wf_auto2.
+  Defined.
+  (* Proof above is 28 LOC *)
+
+  (*
+      Γ ⊢ ∀z.(g z = f z) ∧ P (f x) → ∃y. P (g y)
+  *)
+  Lemma running :
+    Γ ⊢ (all, (g =ml f)) and P $ f^{evar:0 ↦ x} ---> 
+        ex, (P $ g).
+  Proof.
+    mlIntro "H".
+    mlDestructAnd "H" as "H1" "H2". mlSpecialize "H1" with x.
+    mlExists x. mlSimpl.
+    rewrite [P^{evar:0↦x}]evar_open_closed;[wf_auto2|]. (* <- 1 well-formedness constraint *)
+    mlRewriteBy "H1" at 1.
+    mlExact "H2".
+  Defined.
+  (* Proof above is 6 LOC *)
+
+End running.
+
+Section functional_subst.
+  Notation definedness_theory := Theories.Definedness_Syntax.theory.
+  Notation definedness_syntax := Theories.Definedness_Syntax.Syntax.
+  Context
+    {Σ         : Signature}
+    {defsyntax : definedness_syntax}
+    (Γ         : Theory)
+    (HΓ        : definedness_theory ⊆ Γ).
+
+  Context
+    (φ t : Pattern)
+    (wfφ : well_formed (ex, φ))
+    (mfφ : mu_free φ)
+    (wft : well_formed t).
+
+  (* this is the dual version of Lemma 61 in
+     https://fsl.cs.illinois.edu/publications/chen-rosu-2019-tr.pdf
+
+    Γ ⊢ φ[t/x] ∧ (∃z. t = z) → ∃x.φ
+   *)
+  Lemma exists_functional_subst :
+    Γ ⊢ φ^[evar:0↦t] and is_functional t ---> (ex , φ).
+  Proof.
+    remember (fresh_evar (φ $ t)) as Zvar.
+    remember (patt_free_evar Zvar) as Z.
+
+    (* assertions about well-formedness *)
+    assert (well_formed Z) as WFZ.
+    { shelve. }
+
+    assert (well_formed (instantiate (ex , φ) t)) as WF1. {
+      shelve.
+    }
+    assert (well_formed (instantiate (ex , φ) Z)) as WF2. {
+      shelve.
+    }
+    assert (well_formed (ex, φ)) as WFEX.
+    { shelve. }
+    (****)
+
+
+    pose proof (EQ := BasicProofSystemLemmas.Ex_quan Γ φ Zvar WFEX).
+    (* change constraint in EQ. *)
+    use AnyReasoning in EQ.
+    epose proof (PC := prf_conclusion Γ (patt_equal t Z) (instantiate (ex , φ) (patt_free_evar Zvar) ---> ex , φ) AnyReasoning ltac:(shelve) _ EQ).
+
+    assert (Γ ⊢ patt_equal t Z ---> (ex , φ) ^ [t] ---> ex , φ) as HSUB.
+    {
+      epose proof (EE := equality_elimination_proj Γ t Z φ HΓ
+                                               mfφ wft WFZ _ _).
+
+      epose proof (PSP := prf_strenghten_premise Γ ((patt_equal t Z) and (instantiate (ex , φ) Z))
+                                                 ((patt_equal t Z) and (instantiate (ex , φ) t))
+                                                 (ex , φ) _ _ _).
+      eapply MP.
+      2: useBasicReasoning; apply and_impl.
+      2,3,4: shelve.
+      eapply MP.
+      2: eapply MP.
+      3: useBasicReasoning; exact PSP.
+      * unshelve (epose proof (AI := and_impl' Γ (patt_equal t Z) (φ^[evar: 0 ↦ Z]) (ex , φ) _ _ _)).
+        1,2,3: shelve.
+        unfold instantiate.
+        eapply MP. 2: useBasicReasoning; exact AI.
+        rewrite <- HeqZ in PC.
+        exact PC.
+      * apply and_drop. 1-3: shelve.
+        unshelve(epose proof (AI := and_impl' Γ (patt_equal t Z) (instantiate (ex , φ) t) (instantiate (ex , φ) Z) _ _ _)).
+        1-3: shelve.
+        eapply MP. 2: useBasicReasoning; exact AI.
+        { exact EE. }
+    }
+
+    eapply (BasicProofSystemLemmas.Ex_gen Γ _ _ Zvar) in HSUB.
+    3: {
+      shelve.
+    }
+    2: { apply pile_any. }
+
+
+    (* simplifications *)
+    unfold exists_quantify in HSUB.
+    mlSimpl in HSUB.
+    rewrite -> HeqZ, -> HeqZvar in HSUB.
+    simpl evar_quantify in HSUB.
+    rewrite decide_True in HSUB. reflexivity.
+    rewrite evar_quantify_fresh in HSUB.
+    { shelve. }
+    (****)
+
+
+    eapply MP. 2: useBasicReasoning; apply and_impl'. 2-4: shelve.
+    apply reorder_meta. 1-3: shelve.
+    exact HSUB.
+
+
+  Unshelve.
+    (* 29 well-formedness side conditions *)
+    all: try wf_auto2.
+    (* 2 freshness conditions *)
+    clear. 2: solve_fresh.
+    pose proof (free_evars_bevar_subst φ t 0).
+    pose proof (set_evar_fresh_is_fresh' (free_evars φ ∪ free_evars t)).
+    set_solver.
+  Defined.
+  (* Proof above is ~80 LOC *)
+
+  Lemma running_functional_subst :
+    Γ ⊢ φ^[evar:0↦t] and is_functional t ---> (ex , φ).
+  Proof.
+    mlIntro "H".
+    mlDestructAnd "H" as "H1" "H2".
+    mlDestructEx "H2" as x.
+    mlSimpl. cbn.
+
+    (* Use equality elimination to rewrite under substitution: *)
+    unfold evar_open. rewrite (bevar_subst_not_occur _ _ t). shelve. (*!*)
+    opose proof* (equality_elimination_basic Γ t (patt_free_evar x) 
+      {|pcEvar := x; pcPattern := φ^{evar:0 ↦ x}|}); auto. (*!*)
+    { shelve. }
+    { shelve. }
+    cbn in H.
+    mlApplyMeta H in "H2".
+
+    (* Technical: subst cleanup *)
+    erewrite <-bound_to_free_variable_subst with (m := 1); auto. (*!*)
+    2-4: shelve.
+    erewrite <-bound_to_free_variable_subst with (m := 1); auto. (*!*)
+    2-3: shelve.
+    (****)
+
+    mlDestructAnd "H2" as "H2_1" "H2_2".
+    mlExists x. mlApply "H2_1". mlAssumption.
+
+
+  Unshelve. (* These all come from manual application of lemmas (marked with !) *)
+    (* 5 well-formedness constraints *)
+    1-5,7: wf_auto2.
+    (* 1 mu_free contraint *)
+    by apply mu_free_bevar_subst.
+    (* 2 freshness constraints *)
+    fm_solve. fm_solve.
+  Defined.
+  (* Proof above is ~30 LOC *)
+
+End functional_subst.
