matching-logic/src/Evaluation/tutorial.v
@@ -1,0 +1,190 @@
+
+(* What follows is a minimal example of how to use the ProofMode. *)
+
+From MatchingLogic Require Import
+    Syntax
+    ProofSystem
+    ProofMode.MLPM
+.
+
+Import MatchingLogic.Syntax.Notations.
+
+From stdpp Require Import base.
+From Coq Require Import String.
+
+Section tutorial.
+
+Context {Σ : Signature}
+        {Γ : Theory}
+        (ϕ : Pattern)
+        (wfϕ : well_formed ϕ).
+
+Open Scope string_scope.
+
+Open Scope string_scope.
+Open Scope ml_scope.
+
+(* Below we prove that in matching logic, ϕ -> ϕ for any pattern ϕ. *)
+Example phi_implies_phi :
+    Γ ⊢ ϕ ---> ϕ.
+Proof.
+  mlIntro "H".
+  mlExact "H".
+Qed.
+
+(* We can also work with conjunction and disjunction. *)
+Import MatchingLogic.DerivedOperators_Syntax.Notations.
+
+Context (ϕ₁ : Pattern)
+        (wfϕ₁ : well_formed ϕ₁)
+        (ϕ₂ : Pattern)
+        (wfϕ₂ : well_formed ϕ₂).
+
+Example and_or :
+    Γ ⊢ ϕ₁ and ϕ₂ ---> ϕ₁ or ϕ₂
+.
+Proof.
+    mlIntro "H".
+    (* we have tactics like:
+        * [mlDestructAnd]
+        * [mlDestructOr]
+        * [mlLeft]
+        * [mlRight]
+        * [mlSplitAnd]
+       which work similarly to their Coq counterparts
+     *)
+
+    mlDestructAnd "H" as "H1" "H2".
+    mlLeft.
+    mlExact "H1".
+Qed.
+
+Context (ϕ₃ : Pattern)
+        (wfϕ₃ : well_formed ϕ₃)
+        (ϕ₄ : Pattern)
+        (wfϕ₄ : well_formed ϕ₄).
+
+Example use_rewrite :
+    Γ ⊢ ϕ₁ <---> ϕ₂ ->
+    (* The [$] operator is an application. *)
+    Γ ⊢ (ϕ₃ $ ϕ₁ $ ϕ₄) <---> (ϕ₃ $ ϕ₂ $ ϕ₄)
+.
+Proof.
+    intros H.
+    (* Notice that now we have a meta-level assumption [H]. *)
+
+    (* We can use [H] to rewrite the first occurrence of [ϕ₁] to [ϕ₂]. *)
+    mlRewrite H at 1.
+    (* Now the goal is provable by propositional reasoning. *)
+    mlSplitAnd.
+    * mlIntro "H". mlExact "H".
+    * mlIntro "H". mlExact "H".
+Qed.
+
+(* We can also use definedness and equality.
+   To do so, we have to assume that the signature contains a definedness symbol,
+   and the theory a definedness axiom.
+   Otherwise, the signature and axiom can be arbitrary.
+*)
+
+From MatchingLogic Require Import
+    Theories.Definedness_Syntax
+    Theories.Definedness_ProofSystem
+.
+Import Theories.Definedness_Syntax.Notations.
+Open Scope ml_scope.
+Open Scope string_scope.
+
+(* Obviously, without the definedness symbol, we cannot use equality. *)
+Fail Example use_rewriteBy :
+    Γ ⊢ (ϕ₁ $ ϕ₄ =ml ϕ₂ $ ϕ₄ ) ---> (ϕ₁ =ml ϕ₂) ---> ((ϕ₃ $ ϕ₁ $ ϕ₄) <---> (ϕ₃ $ ϕ₂ $ ϕ₄))
+.
+
+(* The typeclass [Definedness_Syntax.Syntax] ensures the presence of the definedness symbol
+   in the (implicit) signature Σ.
+ *)
+Context {syntax : Definedness_Syntax.Syntax}.
+
+Example use_rewriteBy :
+    Γ ⊢ (ϕ₁ $ ϕ₄ =ml ϕ₂ $ ϕ₄) ---> (ϕ₁ =ml ϕ₂) ---> ((ϕ₃ $ ϕ₁ $ ϕ₄) <---> (ϕ₃ $ ϕ₂ $ ϕ₄))
+.
+Proof.
+    mlIntro "H1". mlIntro "H2".
+
+    (* We can rewrite using an equality from the local context. *)
+    mlRewriteBy "H1" at 1.
+    {
+        (* There is an obligation we do not know how to solve. What does that mean? *)
+        unfold theory, named_axioms, NamedAxioms.theory_of_NamedAxioms, axiom. simpl.
+        (* We are missing a Definedness axiom. *)
+        admit.
+    }
+Abort.
+
+Context {HΓ : Definedness_Syntax.theory ⊆ Γ}.
+
+Example use_rewriteBy :
+    Γ ⊢ (ϕ₁ $ ϕ₄ =ml ϕ₂ $ ϕ₄ ) ---> (ϕ₁ =ml ϕ₂) ---> ((ϕ₃ $ ϕ₁ $ ϕ₄) <---> (ϕ₃ $ ϕ₂ $ ϕ₄))
+.
+Proof.
+    mlIntro "H1". mlIntro "H2".
+
+    (* We can rewrite using an equality from the local context. *)
+    mlRewriteBy "H1" at 1.
+    (* Now the obligation was solved automatically *)
+
+    mlSplitAnd; mlIntro "H"; mlExact "H".
+Defined.
+
+
+(*
+   We now demonstrate how to use local hypotheses that are implications.
+*)
+Example use_mlApply :
+    Γ ⊢ (ϕ₁ ---> ϕ₂ $ ϕ₃) ---> (ϕ₂ $ ϕ₃ ---> ϕ₃) ---> (ϕ₁ ---> ϕ₃).
+Proof.
+    mlIntro "H1". mlIntro "H2". mlIntro "H3".
+    (* replace the goal with the premise of "H2", since the goal is exactly
+       the conclusion of "H2" *)
+    mlApply "H2".
+    (* Alternatively: replace "H3" with the conclusion of "H1", since "H3" is
+                      the premise of "H1". *)
+    (* mlApply "H1" in "H3". *)
+
+    mlApply "H1".
+    mlExact "H3".
+Defined.
+
+Context (ψ : Pattern)
+        (wfψ : well_formed (ex, ψ)).
+
+(*
+   What if we have a matching logic implication in a Coq hypothesis
+   or in a lemma? There is `mlApplyMeta` for that.
+*)
+Example use_mlApplyMeta :
+    Γ ⊢ ϕ₁ ---> ((ex, ψ) $ ϕ₂) ---> ϕ₃ ---> (ex, (ψ $ ϕ₂)).
+Proof.
+    mlIntro "H1". mlIntro "H2". mlIntro "H3".
+
+    Check Prop_ex_left.
+    (*
+        Prop_ex_left
+        : ∀ (Γ : Theory) (ϕ ψ : Pattern),
+            well_formed (ex , ϕ)
+            → well_formed ψ
+            → Γ ⊢i (ex , ϕ) $ ψ ---> (ex , ϕ $ ψ) using BasicReasoning
+    *)
+    mlApplyMeta Prop_ex_left.
+    (* Did you notice that [mlApplyMeta] automatically instantiated
+       all the preconditions of the lemma?
+       That is, without some magic happening on the background,
+       one would need to manualy specify them,
+       and solve the well-formedness subgoals.
+    *)
+    mlExact "H2".
+Defined.
+
+Close Scope ml_scope.
+Close Scope string_scope.
+Close Scope list_scope.
